pulse/examples/dsls/mini_steel/tests/Pulse.Tests.fst
@@ -4,21 +4,32 @@ open Pulse.Steel.Wrapper
 open Pulse.Syntax
 open Pulse.Main
 
-// %splice_t[foo] (main (Tm_Constant (Bool true)) Tm_Emp)
-// %splice_t[bar] (check_bar ())
-// %splice_t[baz] (check_baz ())
+%splice_t[foo] (parse_and_check "true")
 
-let foo_s = "true"
-let bar_s = "
-fun (n:Pulse.Steel.Wrapper.erased) (r1:Pulse.Steel.Wrapper.ref) (x:Pulse.Steel.Wrapper.u32) (r2:Pulse.Steel.Wrapper.ref) \
-  {Pulse.Steel.Wrapper.pts_to r1 n * Pulse.Steel.Wrapper.pts_to r2 n} -> \
-    Pulse.Steel.Wrapper.write (n, r2, x) \
-"
+%splice_t[bar] (parse_and_check "\
+  fun (n:Pulse.Steel.Wrapper.erased) \
+      (r1:Pulse.Steel.Wrapper.ref) \
+      (x:Pulse.Steel.Wrapper.u32) \
+      (r2:Pulse.Steel.Wrapper.ref) \
+   {Pulse.Steel.Wrapper.pts_to r1 n * Pulse.Steel.Wrapper.pts_to r2 n} -> \
+      Pulse.Steel.Wrapper.write (n, r2, x) \
+  ")
 
-let baz_s = "fun (n:Pulse.Steel.Wrapper.erased) (r:Pulse.Steel.Wrapper.ref) { Pulse.Steel.Wrapper.pts_to r n } -> let x:Pulse.Steel.Wrapper.u32 = Pulse.Steel.Wrapper.read (n, r); Pulse.Steel.Wrapper.write (n, r, x)"
-
-%splice_t[foo] (parse_and_check foo_s)
-%splice_t[bar] (parse_and_check bar_s)
-
+//Bound variable escapes scope
 [@@ expect_failure]
-%splice_t[baz] (parse_and_check baz_s)
+%splice_t[baz] (parse_and_check  "\
+   fun (n:Pulse.Steel.Wrapper.erased) \
+       (r:Pulse.Steel.Wrapper.ref) \
+         { Pulse.Steel.Wrapper.pts_to r n } -> \
+         let x:Pulse.Steel.Wrapper.u32 = Pulse.Steel.Wrapper.read_alt (n, r); \
+         Pulse.Steel.Wrapper.write (n, r, x) \
+   ")
+
+
+%splice_t[baz_alt] (parse_and_check  "\
+   fun (n:Pulse.Steel.Wrapper.erased) \
+       (r:Pulse.Steel.Wrapper.ref) \
+         { Pulse.Steel.Wrapper.pts_to r n } -> \
+         let x:Pulse.Steel.Wrapper.u32 = Pulse.Steel.Wrapper.read_alt (n, r); \
+         Pulse.Steel.Wrapper.write_alt (n, r, x) \
+   ")
